code/experimental/rsa/Hacl.Impl.Montgomery.fst
@@ -46,68 +46,85 @@ let mod_inv_u64 n0 =
     uv.(size 1)
   )
 
-val bn_mult_by_limb_addj_carry:
-  #aLen:size_nat -> aaLen:size_t{v aaLen == aLen} -> a:lbignum aLen ->
-  l:uint64 -> carry:uint64 -> i:size_t{v i <= aLen} -> j:size_t ->
-  resLen:size_t{aLen + v j < v resLen} -> res:lbignum (v resLen) -> Stack uint64
-  (requires (fun h -> live h a /\ live h res /\ disjoint res a))
-  (ensures (fun h0 _ h1 -> preserves_live h0 h1 /\ modifies1 res h0 h1))
-  [@"c_inline"]
-let rec bn_mult_by_limb_addj_carry #aLen aaLen a l carry i j resLen res =
-  let ij = add #SIZE i j in
-  if (i <. aaLen) then begin
-    let res_ij = res.(ij) in
-    let (carry', res_ij) = bn_mul_by_limb_addj_f a.(i) l carry res_ij in
-    res.(ij) <- res_ij;
-    bn_mult_by_limb_addj_carry aaLen a l carry' (add #SIZE i (size 1)) j resLen res end
-  else begin
-    let res_ij = res.(ij) in
-    let (c', res_ij) = addcarry_u64 (u64 0) res_ij carry in
-    res.(ij) <- res_ij;
-    c' end
+val mont_reduction_f:
+  #nLen:size_nat -> #rLen:size_nat{nLen < rLen} ->
+  nnLen:size_t{v nnLen == nLen} ->
+  rrLen:size_t{v rrLen == rLen /\ nLen + rLen < max_size_t} ->
+  c:lbignum (nLen + rLen) -> n:lbignum nLen -> nInv_u64:uint64 ->
+  carry:lbignum 1 -> i:size_t{v i < nLen} -> Stack unit
+  (requires (fun h -> live h c /\ live h n /\ live h carry /\ disjoint c n))
+  (ensures (fun h0 _ h1 -> preserves_live h0 h1 /\ modifies2 carry c h0 h1))
+  [@ "substitute"]
+let mont_reduction_f #nLen #rLen nnLen rrLen c n nInv_u64 carry i =
+  let ci = c.(i) in
+  let qi = mul_mod #U64 nInv_u64 ci in
+  (* FIX: res = res + limb * bn * beta ^ i *)
+  bn_mult_by_limb_addj nnLen n qi i (add #SIZE nnLen rrLen) c carry;
+  let c_ni =  c.(add #SIZE nnLen i) in
+  let (c1, c_ni) = addcarry_u64 (u64 0) c_ni carry.(size 0) in
+  c.(add #SIZE nnLen i) <- c_ni;
+  let c_ni1 = c.(add #SIZE (add #SIZE nnLen i) (size 1)) in
+  c.(add #SIZE (add #SIZE nnLen i) (size 1)) <- add_mod #U64 c_ni1 c1
 
 val mont_reduction_:
   #nLen:size_nat -> #rLen:size_nat{nLen < rLen} ->
   nnLen:size_t{v nnLen == nLen} ->
   rrLen:size_t{v rrLen == rLen /\ nLen + rLen < max_size_t} ->
   c:lbignum (nLen + rLen) -> n:lbignum nLen -> nInv_u64:uint64 ->
-  i:size_t{v i < rLen}  -> Stack unit
-    (requires (fun h -> live h c /\ live h n /\ disjoint c n))
-    (ensures (fun h0 _ h1 -> preserves_live h0 h1 /\ modifies1 c h0 h1))
+  carry:lbignum 1 -> Stack unit
+  (requires (fun h -> live h c /\ live h n /\ live h carry /\ disjoint c n))
+  (ensures (fun h0 _ h1 -> preserves_live h0 h1 /\ modifies2 carry c h0 h1))
+  [@ "substitute"]
+let mont_reduction_ #nLen #rLen nnLen rrLen c n nInv_u64 carry =
+  let h0 = FStar.HyperStack.ST.get() in
+  loop2_simple #h0 #uint64 #uint64 #1 #(nLen + rLen) nnLen carry c
+  (fun i ->
+    carry.(size 0) <- u64 0;
+    mont_reduction_f #nLen #rLen nnLen rrLen c n nInv_u64 carry i
+  );
+  let ci = c.(nnLen) in
+  let qi = mul_mod #U64 nInv_u64 ci in
+  bn_mult_by_limb_addj nnLen n qi nnLen (add #SIZE nnLen rrLen) c carry;
+  let c_ni =  c.(add #SIZE nnLen nnLen) in
+  let c1 = carry.(size 0) in
+  c.(add #SIZE nnLen nnLen) <- add_mod #U64 c_ni c1
+
+val mont_reduction_a:
+  #nLen:size_nat -> #rLen:size_nat{nLen < rLen} ->
+  nnLen:size_t{v nnLen == nLen} ->
+  rrLen:size_t{v rrLen == rLen /\ nLen + rLen < max_size_t} ->
+  c:lbignum (nLen + rLen) -> n:lbignum nLen -> nInv_u64:uint64 -> Stack unit
+  (requires (fun h -> live h c /\ live h n /\  disjoint c n))
+  (ensures (fun h0 _ h1 -> preserves_live h0 h1 /\ modifies1 c h0 h1))
   [@"c_inline"]
-let rec mont_reduction_ #nLen #rLen nnLen rrLen c n nInv_u64 i =
-  if (i <. nnLen) then begin
-    let ci = c.(i) in
-    let qi = mul_mod #U64 nInv_u64 ci in
-    let carry = bn_mult_by_limb_addj_carry nnLen n qi (u64 0) (size 0) i (add #SIZE nnLen rrLen) c in
-    let c_i1 = c.(add #SIZE (add #SIZE nnLen i) (size 1)) in
-    c.(add #SIZE (add #SIZE nnLen i) (size 1)) <- add_mod #U64 c_i1 carry;
-    mont_reduction_ nnLen rrLen c n nInv_u64 (add #SIZE i (size 1))
-  end else begin
-    let ci = c.(i) in
-    let qi = mul_mod #U64 nInv_u64 ci in
-    let carry = bn_mult_by_limb_addj_carry nnLen n qi (u64 0) (size 0) i (add #SIZE nnLen rrLen) c in ()
-  end
+let mont_reduction_a #nLen #rLen nnLen rrLen c n nInv_u64 =
+  alloc #uint64 #unit #1 (size 1) (u64 0) [BufItem n] [BufItem c]
+  (fun h0 _ h1 -> True)
+  (fun carry ->
+    mont_reduction_ #nLen #rLen nnLen rrLen c n nInv_u64 carry
+  )
 
 val mont_reduction:
   #nLen:size_nat -> #rLen:size_nat{nLen < rLen} ->
   nnLen:size_t{v nnLen == nLen} ->
   rrLen:size_t{v rrLen == rLen /\ nLen + rLen < max_size_t} ->
   n:lbignum nLen -> nInv_u64:uint64 ->
-  c:lbignum (nLen + nLen) -> tmp:lbignum (nLen + rLen) -> res:lbignum nLen ->
-  Stack unit
-    (requires (fun h -> live h n /\ live h c /\ live h tmp /\ live h res /\ disjoint tmp n))
-    (ensures (fun h0 _ h1 -> preserves_live h0 h1 /\ modifies2 res tmp h0 h1))
+  c:lbignum (nLen + nLen) -> tmp:lbignum (nLen + rLen) ->
+  res:lbignum nLen -> Stack unit
+  (requires (fun h -> live h n /\ live h c /\ live h tmp /\ live h res /\ disjoint tmp n))
+  (ensures (fun h0 _ h1 -> preserves_live h0 h1 /\ modifies2 res tmp h0 h1))
   [@"c_inline"]
 let mont_reduction #nLen #rLen nnLen rrLen n nInv_u64 c tmp res =
   let nLen2 = add #SIZE nnLen nnLen in
-  let tmp' = Buffer.sub #uint64 #(nLen +rLen) #(v nLen2) tmp (size 0) nLen2 in
-  copy nLen2 c tmp';
+  let tmp1 = Buffer.sub #uint64 #(nLen +rLen) #(v nLen2) tmp (size 0) nLen2 in
+  copy nLen2 c tmp1;
   tmp.(nLen2) <- u64 0;
-  mont_reduction_ nnLen rrLen tmp n nInv_u64 (size 0);
+  mont_reduction_a nnLen rrLen tmp n nInv_u64;
   //bn_rshift rLen2 tmp (mul #SIZE (size 64) rrLen) tmp; // tmp = tmp / r
-  let tmp' = Buffer.sub #uint64 #(nLen + rLen) #nLen tmp rrLen nnLen in
-  copy nnLen tmp' res
+  let tmp1 = Buffer.sub #uint64 #(nLen + rLen) #nLen tmp rrLen nnLen in
+  copy nnLen tmp1 res
+
+#reset-options "--lax"
 
 val to_mont:
   #nLen:size_nat -> #rLen:size_nat{nLen < rLen} ->
@@ -128,11 +145,9 @@ let to_mont #nLen #rLen nnLen rrLen pow2_i n nInv_u64 r2 a st_kara aM =
   let c = Buffer.sub #uint64 #(v stLen) #(v cLen) st_kara (size 0) cLen in
   karatsuba pow2_i nnLen a r2 st_kara; // c = a * r2
   let tmp = Buffer.sub #uint64 #(v stLen) #(nLen + rLen) st_kara cLen (add #SIZE nnLen rrLen) in
-  assume (disjoint tmp n);
-  let h0 = FStar.HyperStack.ST.get() in
-  mont_reduction #nLen #rLen nnLen rrLen n nInv_u64 c tmp aM; // aM = c % n
-  let h1 = FStar.HyperStack.ST.get() in
-  assume (modifies2 aM st_kara h0 h1)
+  mont_reduction #nLen #rLen nnLen rrLen n nInv_u64 c tmp aM // aM = c % n
+
+#reset-options "--z3rlimit 30"
 
 val from_mont:
   #nLen:size_nat -> #rLen:size_nat{nLen < rLen} ->
@@ -148,9 +163,9 @@ val from_mont:
 let from_mont #nLen #rLen nnLen rrLen pow2_i n nInv_u64 aM tmp a =
   let tmpLen = add #SIZE nnLen rrLen in
   fill tmpLen tmp (u64 0);
-  let tmp' = Buffer.sub #uint64 #(v tmpLen) #nLen tmp (size 0) nnLen in
-  copy nnLen aM tmp';
-  mont_reduction_ nnLen rrLen tmp n nInv_u64 (size 0);
+  let tmp1 = Buffer.sub #uint64 #(v tmpLen) #nLen tmp (size 0) nnLen in
+  copy nnLen aM tmp1;
+  mont_reduction_a nnLen rrLen tmp n nInv_u64;
   //bn_rshift rLen2 tmp (mul #SIZE (size 64) rrLen) tmp; // tmp = tmp / r
-  let tmp' = Buffer.sub #uint64 #(v tmpLen) #nLen tmp rrLen nnLen in
-  copy nnLen tmp' a
+  let tmp1 = Buffer.sub #uint64 #(v tmpLen) #nLen tmp rrLen nnLen in
+  copy nnLen tmp1 a
